%%% Local Variables:
%%% TeX-master: "Proofs"
%%% End:
\probsec{~\ref{sec:compl-set-diff}}
\begin{enumerate}
    \item Let $A = \Z$, $B = \{n \in \Z \mid n \text{ is even}\}$, $C = \{0\}$, and $D = \{x \in \R \mid x <0\}$. For all of the following, make sure to prove your answer.
  \begin{enumerate}
      \item What is $A - B$?
      \item What is $B - A$?
      \item What is $A - (B - C)$?
      \item What is $A - D$?
      \item What is $(A \cap B) - (C \cup D)$?
  \end{enumerate}

    \item Determine which of the following statements is true.
  \begin{enumerate}
      \item $\forall X \subset \N$, $\exists Y \subset X$ such that $\# (X - Y) = 1$.
      \item $\forall X \subset \N$, $\exists Y \subset \N$ such that $\# (Y - X) = 1$.
      \item $\forall X \subset \N$, $\exists Y \subset \Z$ such that $\# (Y - X) = 1$.
  \end{enumerate}

    \item Let $A$ and $B$ be sets. Prove that $A - B = A \cap B^c$.

    \item Show by example that $A - (B - C) \neq (A - B) - C$.

    \item Prove that $A - B = A - (A \cap B)$.

    \item Prove that $A - B = (A \cup B) - B$.

    \item Show by example that $A - B \neq (A \cup B) - (A \cap B)$.

    \item Prove that $(A \cup B) - (A \cap B) = (A - B) \cup (B - A)$.\sidenote{The expressions on both sides of the equation are often called the \emph{symmetric difference} of $A$ and $B$, written $A \triangle B$.}

    \item Prove that $(A \cap B) \cup (A \cap B^c) = A$.

    \item Prove \Cref{prop:complements}.

    \item The following are the set-theoretic analogues of DeMorgan's Laws.
  \begin{enumerate}
      \item Prove that $(A \cup B)^c = A^c \cap B^c$.
      \item Prove that $(A \cap B)^c = A^c \cup B^c$.
  \end{enumerate}

    \item Show the following by example.
  \begin{enumerate}
      \item $(A \cup B)^c \neq A^c \cup B^c$ \marginnote{As you have probably guessed, $\neq$ is slightly different than $=$: $=$ means equality always holds, while $\neq$ means that \emph{sometimes} inequality holds. In other words, $\exists A, B$ such that the two sides are unequal.}
      \item $(A \cap B)^c \neq A^c \cap B^c$
  \end{enumerate}
\end{enumerate}
